meow

TAPLFormalization/02.5-alpha_reduction/alpha_theorem.lean
@@ -1,4 +1,4 @@
-import TAPLFormalization.«02-lambda».Semantics
+import TAPLFormalization.«02.5-alpha_reduction».AST
 
 def Change (x : String) (x' : String) (s : Env) : Env :=
   match s x, s x' with
@@ -49,7 +49,7 @@ lemma SubstIsSane: ∀ t: LambdaTerm, ∀ x : String, t.Subst x x = t := by
   case abs u body ih =>
     by_cases h : u = x <;> simp_all [LambdaTerm.Subst]
 
-lemma ChangeOfChanges : ∀t : LambdaTerm, ∀ x x' : String, ∀ d: Nat, ∀ levels: Env, (x∉ FV t) ∨ (∃ v, levels x = some v) →  (x'∉ FV t)∨  (∃ v, levels x' = some v) → removeNames' d (Change x x' levels) (t.Subst x x') = removeNames' d levels t := by
+lemma ChangeOfChanges : ∀t : LambdaTerm, ∀ x x' : String, ∀ d: Nat, ∀ levels: Env, (x∉ FV t) ∨ (∃ v, levels x = some v) →  (x'∉ FV t) ∨  (∃ v, levels x' = some v) → removeNames' d (Change x x' levels) (t.Subst x x') = removeNames' d levels t := by
   intro t x x'
   induction t
   case var y =>
@@ -213,11 +213,6 @@ theorem AlphaConversion' : ∀ t₁ t₂ : LambdaTerm, ∀ d:ℕ, ∀ levels : E
       simp_all
       exact ih t' (d+1) (levels.insert x d) a
 
-theorem AlphaConversion : ∀ t₁ t₂ : LambdaTerm, Alpha t₁ t₂ → removeNames t₁ = removeNames t₂ := by
-  intro t₁ t₂ A
-  rw[removeNames]
-  exact AlphaConversion' t₁ t₂ 0 Env.empty A
-
 @[simp]
 def ValidEnv (levels : Env) (d : ℕ) : Prop :=
   -- 1. Injectivity
@@ -225,10 +220,163 @@ def ValidEnv (levels : Env) (d : ℕ) : Prop :=
   -- 2. Freshness
   (∀ x v, levels x = some v → v < d)
 
+lemma PreservationValid (levels: Env) (d:ℕ) (x:String): ValidEnv levels d → ValidEnv (levels.insert x d) (d+1):= by
+  grind[ValidEnv, Env.insert]
+
 lemma Transposition:∀levels:Env, ∀x x': String,∀ d: ℕ, (Change x x' (levels.insert x' d)).erase x' = (levels.insert x d).erase x' := by
   intro levels x x' d
   funext k
   by_cases h_kx : x = x' <;> by_cases h_kx : k = x <;> by_cases h_kx' : k = x' <;> cases hx : levels x <;> cases hx' : levels x' <;> simp_all [Change, Ne.symm]
+
+
+
+
+abbrev LinkedState := LambdaTerm × LambdaTerm × Env × Env × ℕ
+
+inductive Step : LinkedState → LinkedState → Prop where
+  | abs_step (arg₁ arg₂ : String) (body₁ body₂ : LambdaTerm) (level₁ level₂ : Env) (d : ℕ) :
+      Step (.abs arg₁ body₁, .abs arg₂ body₂, level₁, level₂, d) (body₁,body₂, level₁.insert arg₁ d, level₂.insert arg₂ d, d+1)
+  | app_left (t₁₂ t₁₁ t₂₁ t₂₂ : LambdaTerm) (level₁ level₂ : Env) (d : ℕ) :
+      Step (.app t₁₁ t₁₂,.app t₂₁ t₂₂, level₁, level₂, d) (t₁₁,t₂₁, level₁, level₂, d)
+  | app_right (t₁₂ t₁₁ t₂₁ t₂₂ : LambdaTerm) (level₁ level₂ : Env) (d : ℕ) :
+      Step (.app t₁₁ t₁₂,.app t₂₁ t₂₂, level₁, level₂, d) (t₁₂,t₂₂, level₁, level₂, d)
+
+inductive RealPath : List LinkedState → Prop where
+  | singleton (x₁ x₂: String) (level₁ level₂: Env) (d:Nat) : RealPath [(.var x₁, .var x₂, level₁, level₂, d)]
+  | cons (s₁ s₂ : LinkedState) (rest : List LinkedState)
+      (hStep : Step s₁ s₂)
+      (hRest : RealPath (s₂ :: rest)) : RealPath (s₁ :: s₂ :: rest)
+
+@[simp]
+def avoidsAbsX (x : String) : List LinkedState → Prop
+  | [] => True
+  | (t, _, _, _, _) :: rest => (∀ body, t ≠ .abs x body) ∧ avoidsAbsX x rest
+
+lemma free_implies_path (t₁ : LambdaTerm) (x : String) : ∀ t₂ level₁ level₂ d, removeNames' d level₁ t₁ = removeNames' d level₂ t₂ →
+    x ∈ FV t₁ →
+      ∃ (path : List LinkedState),
+        path.head? = some (t₁, t₂, level₁, level₂, d) ∧
+        RealPath path ∧
+        avoidsAbsX x path ∧
+        ∃ a b c d, path.getLast? = some (.var x, a, b, c, d):= by
+  induction t₁ with
+  | var name =>
+    intro t₂ level₁ level₂ d rh h
+    use [(.var x, t₂, level₁, level₂, d)]
+    simp_all[FV]
+    have ⟨y, m⟩: ∃ y, t₂ = .var y := by
+      cases t₂ with
+      | var y =>
+        exact ⟨y, rfl⟩
+      | abs arg body =>
+        revert rh
+        cases level₁ name <;> intro rh <;> contradiction
+      | app l r =>
+        revert rh
+        cases level₁ name <;> intro rh <;> contradiction
+    rw[m]
+    constructor
+  | abs arg body ih =>
+    intro t₂ level₁ level₂ d rh h
+    simp[FV, Finset.mem_erase] at h
+    rcases h with ⟨h_neq, h_body⟩
+    simp_all
+    cases t₂ <;> try grind[removeNames']
+    rename_i arg₂ body₂
+    have:removeNames' (d + 1) (level₁.insert arg d) body = removeNames' (d + 1) (level₂.insert arg₂ d) body₂:= by
+      simp_all[removeNames']
+    have ⟨path, hHead, hPath, hAvoids, hTail⟩:= ih body₂ (level₁.insert arg d) (level₂.insert arg₂ d) (d+1) this
+    cases path with
+    | nil => simp at hHead
+    | cons s rest =>
+      use (.abs arg body, .abs arg₂ body₂, level₁, level₂, d) :: (body, body₂, level₁.insert arg d, level₂.insert arg₂ d, d + 1) :: rest
+      simp_all
+      constructor
+      constructor
+      constructor
+      exact hPath
+      grind
+  | app t₁ t₂ ih₁ ih₂ =>
+    intro t₂ level₁ level₂ d rh h
+    cases t₂ <;> try grind[removeNames']
+    simp only [FV, Finset.mem_union] at h
+    rename_i t₂₁ t₂₂
+    cases h with
+    | inl h₁ =>
+      simp_all
+      have :  removeNames' d level₁ t₁ = removeNames' d level₂ t₂₁ := by grind
+      have ⟨path, hHead, hPath, hAvoids, hTail⟩ := ih₁ t₂₁ level₁ level₂ d this
+      cases path with
+      | nil => simp at hHead
+      | cons s rest =>
+        use (.app t₁ t₂, .app t₂₁ t₂₂, level₁, level₂, d) :: (t₁, t₂₁, level₁, level₂, d) :: rest
+        simp_all
+        constructor
+        constructor
+        exact hPath
+    | inr h₂ =>
+      simp_all
+      have :  removeNames' d level₁ t₂ = removeNames' d level₂ t₂₂ := by grind
+      have ⟨path, hHead, hPath, hAvoids, hTail⟩ := ih₂ t₂₂ level₁ level₂ d this
+      cases path with
+      | nil => simp at hHead
+      | cons s rest =>
+        use (.app t₁ t₂, .app t₂₁ t₂₂, level₁, level₂, d) :: (t₂, t₂₂, level₁, level₂, d) :: rest
+        simp_all
+        constructor
+        constructor
+        exact hPath
+
+abbrev Invariant (x : String) (state : LinkedState) : Prop :=
+  let (t₁, t₂, level₁, level₂, d) := state
+  level₁ x ≠ level₂ x ∧
+  (∀ y v, level₁ x = some v → level₂ y = some v → x = y) ∧
+  ValidEnv level₁ d ∧
+  ValidEnv level₂ d ∧
+  removeNames' d level₁ t₁ = removeNames' d level₂ t₂
+
+lemma InvariantIsPathInvariant (x : String) :
+    ∀ (path : List LinkedState) (s_start s_end : LinkedState),
+      RealPath path →
+      avoidsAbsX x path →
+      path.head? = some s_start →
+      path.getLast? = some s_end →
+      Invariant x s_start →
+      Invariant x s_end := by
+  intro path
+  induction path
+  · grind
+  · rename_i head tail ih
+    intro start_ end_ rh ah h₁ h₂ inh
+    cases tail with
+    | nil => grind
+    | cons s rest =>
+      have rh': RealPath (s :: rest) := by grind[RealPath]
+      have ah': avoidsAbsX x (s :: rest):= by grind[avoidsAbsX]
+      have hh': (s :: rest).head? = some s := by grind
+      have he': (s :: rest).getLast? = some end_:=by grind
+      have := ih s end_ rh' ah' hh' he'
+      apply this
+      rw[Invariant]
+      have step: Step head s := by
+        cases rh with
+        | cons _ _ _ hStep hRest =>
+          exact hStep
+      have: head=start_:=by grind
+      subst this
+      clear rh' ah' hh' he' ih h₂ this h₁ end_
+      have ⟨t₁₁, t₁₂, level₁₁, level₁₂, d₁⟩:=head
+      have ⟨t₂₁, t₂₂, level₂₁, level₂₂, d₂⟩:=s
+      have ⟨A,B,C,D,E⟩ := inh
+      dsimp only
+      cases step
+      · rename_i arg₁ arg₂
+        grind[avoidsAbsX,ValidEnv, Env.insert,removeNames']
+      · rename_i r₁ r₂
+        grind[removeNames']
+      · rename_i r₁ r₂
+        grind[removeNames']
+
 
 theorem AlphaConversion'' : ∀ t₁ t₂ : LambdaTerm, ∀ d:ℕ, ∀ levels : Env, ValidEnv levels d → removeNames' d levels t₁ = removeNames' d levels t₂ → Alpha t₁ t₂ := by
   intro t₁
@@ -260,27 +408,49 @@ theorem AlphaConversion'' : ∀ t₁ t₂ : LambdaTerm, ∀ d:ℕ, ∀ levels : 
       have I_new : ValidEnv (levels.insert x d) (d + 1) := by
         rcases I with ⟨h_inj, h_fresh⟩
         constructor
-        ·
-          intro y y' v hy hy'
+        · intro y y' v hy hy'
           simp only [Env.insert] at hy hy'
           by_cases h1 : y = x <;> by_cases h2 : y' = x <;> grind
-        ·
-          intro y v hy
+        · intro y v hy
           simp only [Env.insert] at hy
           by_cases h1 : y = x <;> grind
 
       have ih := ih (t'.Subst x x') (d+1) (levels.insert x d) I_new
       rw[R_inner] at ih
 
-      -- x!=x'
-      have h_not_free : x ∉ FV t' := by sorry
+      by_cases h:x=x'
+      · constructor
+        · exact Or.inr h
+        · apply ih
+          rw[h, SubstIsSane]
+      · have h_not_free : x ∉ FV t' := by
+          intro contr
+          have:removeNames' (d + 1) (levels.insert x' d) t'=removeNames' (d + 1) (levels.insert x d) t:= by grind
+          have ⟨path, bh, rh, ah, eh⟩:=free_implies_path t' x t (levels.insert x' d) (levels.insert x d) (d+1) this contr
+          have ⟨a',b',c',d',eh⟩ := eh
+          have inv : Invariant x (t', t, (levels.insert x' d), (levels.insert x d), (d+1)) := by
+            grind[ValidEnv, Env.insert]
+          have ⟨i₁, i₂, i₃, i₄, i₅⟩:=InvariantIsPathInvariant x path (t', t, (levels.insert x' d), (levels.insert x d), (d+1)) (LambdaTerm.var x, a', b', c', d') rh ah bh eh inv
+          cases a' <;> try grind[removeNames']
 
-      have h_bridge : removeNames' (d + 1) (levels.insert x' d) t' = removeNames' (d + 1) (levels.insert x d) (t'.Subst x x') := by
-        have helpA : (x' ∉ FV t' ∨ ∃ v, (levels.insert x' d) x' = some v) := Or.inr ⟨d, by simp [Env.insert]⟩
-        have A_eq := ChangeOfChanges t' x x' (d+1) (levels.insert x' d) (Or.inl h_not_free) helpA
-        rw [←A_eq]
-        have D:= Transposition levels x x' d
-        have C := LevelsUnfree (LambdaTerm.Subst x x' t') x' (d+1) (Change x x' (levels.insert x' d)) (levels.insert x d) (Subst_FV_neq t' x x' h_not_free) D
-        rw [C]
-      grind[Alpha]
+        have h_bridge : removeNames' (d + 1) (levels.insert x' d) t' = removeNames' (d + 1) (levels.insert x d) (t'.Subst x x') := by
+          have helpA : (x' ∉ FV t' ∨ ∃ v, (levels.insert x' d) x' = some v) := Or.inr ⟨d, by simp [Env.insert]⟩
+          have A_eq := ChangeOfChanges t' x x' (d+1) (levels.insert x' d) (Or.inl h_not_free) helpA
+          rw [←A_eq]
+          have D:= Transposition levels x x' d
+          have C := LevelsUnfree (LambdaTerm.Subst x x' t') x' (d+1) (Change x x' (levels.insert x' d)) (levels.insert x d) (Subst_FV_neq t' x x' h_not_free) D
+          rw [C]
+        grind[Alpha]
+
+
     | _ => grind [removeNames']
+
+theorem AlphaConversion : ∀ t₁ t₂ : LambdaTerm, Alpha t₁ t₂ ↔ removeNames t₁ = removeNames t₂ := by
+  intro t₁ t₂
+  constructor
+  · intro A
+    rw[removeNames]
+    exact AlphaConversion' t₁ t₂ 0 Env.empty A
+  · intro A
+    have EmptyIsValid : ValidEnv Env.empty 0 := by simp_all
+    exact AlphaConversion'' t₁ t₂ 0 Env.empty EmptyIsValid A
